work

pancake/semantics/panWorkSetScript.sml
@@ -7,6 +7,8 @@
      * addr:  Used for memory addresses. Pluralised as addrs.
      * ctxt:  Short for "context".
      * m:     Stands for "memory". Pluralised as ms.
+     * s:     Stands for "state". It refers to both the state in panSemTheory,
+              and the state used by working_set. Pluralised also as s.
      * v:     1. Used for Pancake variable names. 2. A Pancake value.
      * ws:    1. Short for "working set". Here, it is usually an upper bound on
               the range of heap addresses that a Pancake program or expression
@@ -110,6 +112,456 @@ End
 
 (* Find an upper bound on the working set of a Pancake program. *)
 
+Datatype:
+  context = <| code      : funname |-> ((varname # shape) list # ('a panLang$prog)) ;
+               be        : bool ;
+               base_addr : 'a word ;
+               ffi       : 'ffi itself |>
+End
+
+Definition context_from_state_def:
+  context_from_state (s:('a, 'ffi) panSem$state) =
+    <| code := s.code ; be := s.be ; base_addr := s.base_addr ; ffi := (:'ffi) |>
+End
+
+Type state = (Type ‘:(varname |-> 'a v) # ('a word -> 'a word_lab)’)
+
+Definition value_range_def:
+  value_range (ctxt:('a, 'ffi) context) e sts =
+    let state (l, m) =
+        <| code      := ctxt.code ;
+           locals    := l ;
+           memory    := m ;
+           memaddrs  := UNIV ;
+           be        := ctxt.be ;
+           ffi       := (ARB : 'ffi ffi_state) ;
+           base_addr := ctxt.base_addr |>
+    in { x | SOME x ∈ IMAGE (λst. eval (state st) e) sts }
+End
+
+Definition working_set_mem_load_def:
+  working_set_mem_load sh addr =
+  (case sh of
+     One => {addr}
+   | Comb shs => working_set_mem_loads shs addr) ∧
+  working_set_mem_loads [] addr = {} ∧
+  working_set_mem_loads (sh::shs) addr =
+    working_set_mem_load sh addr ∪
+    working_set_mem_loads shs (addr + bytes_in_word * n2w (size_of_shape sh))
+Termination
+  WF_REL_TAC ‘measure (λx. case x of
+                             INL (sh, addr) => shape_size sh
+                           | INR (shs, addr) => list_size shape_size shs)’
+End
+
+Definition working_set_mem_stores_def:
+  working_set_mem_stores a [] = {a} ∧
+  working_set_mem_stores a (w::ws) =
+  {a} ∪ working_set_mem_stores (a + bytes_in_word) ws
+End
+
+Definition working_set_exp_def:
+  working_set_exp ctxt ((Const w):'a panLang$exp) (sts:'a state set) = ({}:'a word set) ∧
+  working_set_exp ctxt (Var v) sts = {} ∧
+  working_set_exp ctxt (Label fname) sts = {}  ∧
+  working_set_exp ctxt (panLang$Struct es) sts =
+    FOLDR (λe ws. ws ∪ working_set_exp ctxt e sts) {} es ∧
+  working_set_exp ctxt (Field index e) sts = working_set_exp ctxt e sts ∧
+  working_set_exp ctxt (Load shape src) sts =
+    working_set_exp ctxt src sts ∪
+    BIGUNION { working_set_mem_load shape addr | ValWord addr ∈ value_range ctxt src sts } ∧
+  working_set_exp ctxt (LoadByte e) sts =
+    (let addrs = { addr | ValWord addr ∈ value_range ctxt e sts } in
+      working_set_exp ctxt e sts ∪ addrs) ∧
+  working_set_exp ctxt (Op op es) sts =
+    FOLDR (λe ws. ws ∪ working_set_exp ctxt e sts) {} es ∧
+  working_set_exp ctxt (Panop op es) sts =
+    FOLDR (λe ws. ws ∪ working_set_exp ctxt e sts) {} es ∧
+  working_set_exp ctxt (Cmp cmp e1 e2) sts =
+    working_set_exp ctxt e1 sts ∪ working_set_exp ctxt e2 sts ∧
+  working_set_exp ctxt (Shift sh e n) sts = working_set_exp ctxt e sts ∧
+  working_set_exp ctxt BaseAddr sts = {}
+Termination
+  WF_REL_TAC ‘measure (exp_size ARB o (FST o SND))’
+End
+
+Definition working_set_prog_def:
+  working_set_prog ctxt Skip s = ({}, s) ∧
+  working_set_prog ctxt (Dec v e p) sts =
+  (let ws = working_set_exp ctxt e sts;
+       sts' = { (l |+ (v, val), m)
+              | (l, m) ∈ sts ∧ val ∈ value_range ctxt e sts };
+       (ws', sts'') = working_set_prog ctxt p sts' in
+     (ws ∪ ws', sts'')) ∧
+  working_set_prog ctxt (Assign v e) sts =
+  (let ws = working_set_exp ctxt e sts and
+       sts' = { (l |+ (v, val), m)
+              | (l, m) ∈ sts ∧ val ∈ value_range ctxt e sts} in
+     (ws, sts')) ∧
+  working_set_prog ctxt (Store dst src) sts =
+  (let ws = working_set_exp ctxt dst sts and
+       ws' = working_set_exp ctxt src sts and
+       addrs = { addr | ValWord addr ∈ value_range ctxt dst sts } and
+       vals = value_range ctxt src sts;
+       ws'' = BIGUNION { working_set_mem_stores addr (flatten val)
+                       | addr ∈ addrs ∧ val ∈ vals } and
+       sts' = { (l, THE (mem_stores addr (flatten val) UNIV m))
+       | (l, m) ∈ sts ∧ ValWord addr ∈ value_range ctxt dst sts ∧
+         val ∈ vals } in
+     (ws ∪ ws' ∪ ws'', sts')) ∧
+  working_set_prog ctxt (StoreByte dst src) sts =
+  (let ws = working_set_exp ctxt dst sts and
+       ws' = working_set_exp ctxt src sts and
+       addrs = { addr | ValWord addr ∈ value_range ctxt dst sts };
+       sts' = { (l, THE (mem_store_byte m UNIV ctxt.be addr (w2w w)))
+              | (l, m, addr, w)
+              | (l, m) ∈ sts ∧ addr ∈ addrs ∧
+                ValWord w ∈ value_range ctxt src sts } in
+     (ws ∪ ws' ∪ IMAGE byte_align addrs, sts')) ∧
+  working_set_prog ctxt (Seq c1 c2) s =
+  (let (ws, s') = working_set_prog ctxt c1 s;
+       (ws', s'') = working_set_prog ctxt c2 s' in
+     (ws ∪ ws', s'')) ∧
+  working_set_prog ctxt (If e c1 c2) s =
+  (let ws = working_set_exp ctxt e s and
+       (ws', s') = working_set_prog ctxt c1 s and
+       (ws'', s'') = working_set_prog ctxt c2 s in
+     (ws ∪ ws' ∪ ws'', s' ∪ s'')) ∧
+  (* For the purposes of defining the major theorem below, this is sound because
+     the nice semantics are the same as the semantics for While. This saves us
+     a huge headache, but restricts working_set_prog to finding the bound up until
+     the next While loop. *)
+  working_set_prog ctxt (While _ _) s = ({}, s) ∧
+  working_set_prog ctxt Break s = ({}, s) ∧
+  working_set_prog ctxt Continue s = ({}, s) ∧
+  (* See the note above on the While case. *)
+  working_set_prog ctxt (Call _ _ _) s = ({}, s) ∧
+  (* See the note above on the While case. *)
+  working_set_prog ctxt (ExtCall _ _ _ _ _) s = ({}, s) ∧
+  working_set_prog ctxt (Return e) s = (working_set_exp ctxt e s, s) ∧
+  working_set_prog ctxt (Raise _ e) s = (working_set_exp ctxt e s, s) ∧
+  working_set_prog ctxt Tick s = ({}, s)
+End
+
+Definition working_set_def:
+  working_set p s = FST (working_set_prog (context_from_state s) p {(s.locals, s.memory)})
+End
+
+
+(* Prove the major theorem: that if our bound on the working set of a Pancake
+   program is within the allocated heap, we may replace the semantics with the
+   nicer semantics. *)
+
+Theorem OPT_MMAP_exist:
+  ∀xs es f e.
+    SOME xs = OPT_MMAP f es ∧ MEM e es ⇒
+    ∃x. f e = SOME x
+Proof cheat
+QED
+
+Theorem mem_load_mono:
+  ∀sh dm dm' w m.
+    dm ⊆ dm' ⇒
+    mem_load sh w dm m = mem_load sh w dm' m
+Proof cheat
+QED
+
+Theorem eval_value_range:
+  ∀s e x.
+    eval s e = SOME x ⇒
+    x ∈ value_range (context_from_state s) e {(s.locals,s.memory)}
+Proof
+  recInduct eval_ind
+  >> rpt strip_tac
+  >> gvs[eval_def, value_range_def, context_from_state_def, AllCaseEqs()]
+  >- (pop_assum $ assume_tac o GSYM >> simp[]
+      >> match_mp_tac OPT_MMAP_cong
+      >> rw[]
+      >> imp_res_tac OPT_MMAP_exist
+      >> metis_tac[])
+  >- (EXISTS_TAC “(Struct vs)” >> rw[])
+  >- (EXISTS_TAC “(ValWord w)” >> rw[]
+      >> fs[mem_load_def]
+      >> cheat)
+  >> cheat
+QED
+
+Theorem working_set_prog_mono:
+  ∀s1 s2. s1 ⊆ s2 ⇒
+          FST (working_set_prog ctxt p s1) ⊆ FST (working_set_prog ctxt p s2)
+Proof cheat
+QED
+
+Theorem evaluate_preserves_state:
+  ∀p s res s1.
+    evaluate (p, s) = (res, s1) ⇒
+    s1.code = s.code ∧
+    s1.be = s.be ∧
+    s1.base_addr = s.base_addr ∧
+    s1.memaddrs = s.memaddrs
+Proof
+  recInduct panSemTheory.evaluate_ind
+  >> rpt conj_tac
+  >> rpt gen_tac
+  >> rpt $ disch_then strip_assume_tac
+  >> rpt gen_tac
+  >> rpt $ disch_then strip_assume_tac
+  >~ [‘While’]
+  >- (qpat_x_assum ‘evaluate (While e c,s) = (res, s1)’ mp_tac
+      >> once_rewrite_tac[evaluate_def]
+      >> TOP_CASE_TAC >> fs[]
+      >> TOP_CASE_TAC >> fs[]
+      >> TOP_CASE_TAC >> fs[]
+      >> strip_tac
+      >> pairarg_tac >> gvs[]
+      >> Cases_on ‘c' = 0w’
+      >> gs[]
+      >> Cases_on ‘s.clock’
+      >> gvs[empty_locals_def, context_from_state_def]
+      >> ‘SUC n ≠ 0’ by rw[]
+      >> gvs[]
+      >> Cases_on ‘res'’
+      >- gvs[context_from_state_def, dec_clock_def]
+      >- (Cases_on ‘x’ >> gvs[context_from_state_def, dec_clock_def, empty_locals_def]))
+  >> fs[evaluate_def]
+  >> gvs[AllCaseEqs(), empty_locals_def, context_from_state_def, dec_clock_def, empty_locals_def, set_var_def]
+  >> rpt (pairarg_tac >> gvs[])
+  >> gvs[AllCaseEqs()]
+QED
+
+Theorem evaluate_preserves_context:
+  ∀p s res s1. evaluate (p, s) = (res, s1) ⇒
+               context_from_state s1 = context_from_state s
+Proof rw[] >> fs[context_from_state_def] >> metis_tac[evaluate_preserves_state]
+QED
+
+Theorem working_set_prog_Seq:
+  ∀p c1 c2 ctxt s s' dm.
+    p = Seq c1 c2 ∧ FST (working_set_prog ctxt p s) ⊆ dm ∧
+    s' = SND (working_set_prog ctxt c1 s) ⇒
+    FST (working_set_prog ctxt c1 s) ⊆ dm ∧
+    FST (working_set_prog ctxt c2 s') ⊆ dm
+Proof rw[] >> fs[working_set_prog_def] >> rpt (pairarg_tac >> gvs[])
+QED
+
+Theorem working_set_prog_If:
+  ∀p e c1 c2 ctxt s dm.
+    p = If e c1 c2 ∧ working_set p s ⊆ s.memaddrs ⇒
+    working_set c1 s ⊆ s.memaddrs ∧
+    working_set c2 s ⊆ s.memaddrs
+Proof
+  rw[working_set_def]
+  >> fs[working_set_prog_def]
+  >> rpt (pairarg_tac >> gvs[])
+QED
+
+Theorem mem_store_nice:
+  ∀w c dm m. c ∈ dm ⇒ mem_store c w dm m = nice_mem_store c w dm m
+Proof rw[mem_store_def, nice_mem_store_def]
+QED
+
+Theorem mem_stores_nice:
+  ∀ws c dm m. working_set_mem_stores c ws ⊆ dm ⇒
+              mem_stores c ws dm m = nice_mem_stores c ws dm m
+Proof
+  Induct
+  >> simp[mem_stores_def, nice_mem_stores_def, working_set_mem_stores_def]
+  >> rw[mem_store_nice]
+QED
+
+Theorem mem_store_byte_nice:
+  ∀m dm be w b.
+     byte_align w ∈ dm ⇒
+     mem_store_byte m dm be w b = nice_mem_store_byte m dm be w b
+Proof
+  rw[mem_store_byte_def, nice_mem_store_byte_def]
+  >> TOP_CASE_TAC >> gvs[]
+QED
+
+Theorem working_set_prog_over_evaluate:
+  ∀c1 s s1 sts sts'.
+    evaluate (c1,s) = (NONE,s1) ∧
+    sts' = SND (working_set_prog (context_from_state s) c1 {(s.locals,s.memory)}) ⇒
+    {(s1.locals,s1.memory)} ⊆ sts'
+Proof
+  recInduct panSemTheory.evaluate_ind
+  >> rpt strip_tac
+  >> simp[working_set_prog_def]
+  >> cheat
+QED
+
+Theorem working_set:
+  ∀p s.
+    working_set p s ⊆ s.memaddrs ⇒
+    evaluate (p, s) = nice_evaluate (p, s)
+Proof
+  recInduct panSemTheory.evaluate_ind
+  >> rpt strip_tac
+  >> simp[Once nice_evaluate_def]
+  >> simp[evaluate_def]
+  (* Dec case *)
+  >- (rpt (TOP_CASE_TAC >> gvs[])
+      >> rpt (pairarg_tac >> gvs[])
+      >> fs[working_set_def]
+      >> fs[working_set_prog_def]
+      >> rpt (pairarg_tac >> gvs[])
+      >> ‘context_from_state (s with locals := s.locals |+ (v, x)) = context_from_state s’
+                             by rw[context_from_state_def] >> gvs[]
+      >> ‘x ∈ value_range (context_from_state s) e {(s.locals, s.memory)}’
+            by metis_tac[eval_value_range]
+      >> Q.ABBREV_TAC ‘A = {(s.locals |+ (v,x),s.memory)}’
+      >> Q.MATCH_ASSUM_ABBREV_TAC ‘working_set_prog (context_from_state s) prog B = (ws',sts'')’
+      >> ‘A ⊆ B’ by (gvs[Abbr ‘A’, Abbr ‘B’, GSPECIFICATION, IN_DEF, SUBSET_DEF]
+                     (* I could not explain to you why this type annotation is necessary. *)
+                     >> EXISTS_TAC “(s.locals, x, s.memory)
+                                    :((mlstring |-> 'a v) # 'a v # ('a word -> 'a word_lab))”
+                     >> gvs[])
+      >> ‘FST (working_set_prog (context_from_state s) prog A) ⊆
+          FST (working_set_prog (context_from_state s) prog B)’
+        by metis_tac[working_set_prog_mono]
+      >> ‘FST (working_set_prog (context_from_state s) prog B) ⊆ s.memaddrs’
+        by rw[]
+      >> metis_tac[SUBSET_TRANS])
+  (* Store case *)
+  >- (TOP_CASE_TAC >> gvs[]
+      >> TOP_CASE_TAC >> gvs[]
+      >> TOP_CASE_TAC >> gvs[]
+      >> TOP_CASE_TAC >> gvs[]
+      >> gs[working_set_def, working_set_prog_def]
+      >> imp_res_tac eval_value_range
+      >> imp_res_tac BIGUNION_SUBSET
+      >> qmatch_assum_abbrev_tac ‘∀Y. Y ∈ Z ⇒ Y ⊆ s.memaddrs’
+      >> ‘working_set_mem_stores c (flatten x) ∈ Z’
+        by (gvs[Abbr ‘Z’, GSPECIFICATION, IN_DEF, SUBSET_DEF]
+            >> EXISTS_TAC “(c, x):('a word # 'a v)”
+            >> gvs[])
+      >> ‘working_set_mem_stores c (flatten x) ⊆ s.memaddrs’
+        by metis_tac[]
+      >> metis_tac[mem_stores_nice])
+  (* StoreByte case *)
+  >- (TOP_CASE_TAC >> gvs[]
+      >> TOP_CASE_TAC >> gvs[]
+      >> TOP_CASE_TAC >> gvs[]
+      >> TOP_CASE_TAC >> gvs[]
+      >> TOP_CASE_TAC >> gvs[]
+      >> TOP_CASE_TAC >> gvs[]
+      >> gs[working_set_def, working_set_prog_def]
+      >> imp_res_tac eval_value_range
+      >> fs[IMAGE_DEF]
+      >> ‘{byte_align c} ⊆ {byte_align x | ValWord x ∈ value_range (context_from_state s) dst {(s.locals,s.memory)}}’
+        by (rw[] >> EXISTS_TAC “c:'a word” >> rw[])
+      >> ‘{byte_align c} ⊆ s.memaddrs’ by metis_tac[SUBSET_TRANS]
+      >> ‘byte_align c ∈ s.memaddrs’ by gvs[]
+      >> metis_tac[mem_store_byte_nice])
+  (* Seq case *)
+  >- (fs[working_set_def]
+      >> imp_res_tac working_set_prog_Seq >> rw[]
+      >> rpt (pairarg_tac >> gvs[]) >> rw[]
+      >> ‘context_from_state s1 = context_from_state s’
+         by metis_tac[evaluate_preserves_context] >> gvs[]
+      >> ‘s1.memaddrs = s.memaddrs’ by metis_tac[evaluate_preserves_state] >> gvs[]
+      >> ‘{(s1.locals, s1.memory)} ⊆
+          SND (working_set_prog (context_from_state s) c1 {(s.locals, s.memory)})’
+        by metis_tac[working_set_prog_over_evaluate]
+      >> ‘FST (working_set_prog (context_from_state s) c2 {(s1.locals, s1.memory)}) ⊆
+          FST (working_set_prog (context_from_state s) c2
+                                (SND (working_set_prog (context_from_state s) c1
+                                                       {(s.locals, s.memory)})))’
+        by metis_tac[working_set_prog_mono]
+      >> ‘FST (working_set_prog (context_from_state s) c2 {(s1.locals, s1.memory)}) ⊆ s.memaddrs’
+        by metis_tac[SUBSET_TRANS]
+      >> metis_tac[])
+  (* If case *)
+  >- (imp_res_tac working_set_prog_If >> rw[]
+      >> rpt (TOP_CASE_TAC >> gvs[]))
+QED
+
+val workset_tac = DEP_PURE_ONCE_REWRITE_TAC [working_set] >> conj_tac;
+
+val _ = export_theory ();
+
+
+(*
+Definition working_set_prog_def:
+  working_set_prog (Skip:'a panLang$prog) (ctxt:('a, 'ffi) context) = (ctxt, {}) ∧
+  working_set_prog (Dec v e p) ctxt =
+    (let ws = working_set_exp e ctxt and
+         values = range e ctxt;
+         lm = { (locals |+ (v, value), memory)
+              | (locals, memory) ∈ ctxt.locals_memory ∧ value ∈ values };
+         ctxt' = ctxt with locals_memory := lm;
+         (ctxt'', ws') = working_set_prog p ctxt' in
+      (ctxt'', ws ∪ ws')) ∧
+  working_set_prog (Assign v e) ctxt =
+    (let ws = working_set_exp e ctxt and
+         values = range e ctxt;
+         lm = { (locals |+ (v, value), memory)
+              | (locals, memory) ∈ ctxt.locals_memory ∧ value ∈ values } in
+      (ctxt with locals_memory := lm, ws)) ∧
+  working_set_prog (Store dst src) ctxt =
+    (let ws = working_set_exp dst ctxt and
+         ws' = working_set_exp src ctxt and
+         addrs = { addr | ValWord addr ∈ range dst ctxt } and
+         values = range src ctxt;
+         lm = { (locals, THE (mem_stores addr (flatten value) UNIV memory))
+              | (locals, memory) ∈ ctxt.locals_memory ∧ addr ∈ addrs ∧
+                value ∈ values} in
+      (ctxt with locals_memory := lm, ws ∪ ws' ∪ addrs)) ∧
+  working_set_prog (StoreByte dst src) ctxt =
+    (let ws = working_set_exp dst ctxt and
+         ws' = working_set_exp src ctxt and
+         addrs = { addr | ValWord addr ∈ range dst ctxt } and
+         ws = { w | ValWord w ∈ range src ctxt };
+         lm = { (locals, THE (mem_store_byte memory UNIV ctxt.be addr (w2w w)))
+              | locals, memory, addr, w
+              | (locals, memory) ∈ ctxt.locals_memory ∧ addr ∈ addrs ∧
+                w ∈ ws} in
+      (ctxt with locals_memory := lm, ws ∪ ws' ∪ addrs)) ∧
+  working_set_prog (Seq c1 c2) ctxt =
+    (let (ctxt', ws) = working_set_prog c1 ctxt;
+        (ctxt'', ws') = working_set_prog c2 ctxt' in
+      (ctxt'', ws ∪ ws')) ∧
+  working_set_prog (If e c1 c2) ctxt =
+    (let ws = working_set_exp e ctxt and
+        (ctxt', ws') = working_set_prog c1 ctxt and
+        (ctxt'', ws'') = working_set_prog c2 ctxt in
+      (context_union ctxt' ctxt'', ws ∪ ws' ∪ ws'')) ∧
+  working_set_prog (While _ _) ctxt = (ctxt, {}) ∧
+  working_set_prog Break ctxt = (ctxt, {}) ∧
+  working_set_prog Continue ctxt = (ctxt, {}) ∧
+  (* See the note above on the While case. *)
+  working_set_prog (Call _ _ _) ctxt = (ctxt, {}) ∧
+  (* See the note above on the While case. *)
+  working_set_prog (ExtCall _ _ _ _ _) ctxt = (ctxt, {}) ∧
+  working_set_prog (Return e) ctxt = (ctxt, working_set_exp e ctxt) ∧
+  working_set_prog (Raise eid e) ctxt = (ctxt, working_set_exp e ctxt) ∧
+  working_set_prog Tick ctxt = (ctxt, {})
+End
+
+
+
+Theorem working_set_exp:
+  ∀s e.
+    working_set_exp (context_from_state s) e {(s.locals, s.memory)} ⊆ s.memaddrs ⇒
+    eval s e = nice_eval s e
+Proof
+  recInduct panSemTheory.eval_ind
+  >> rpt strip_tac
+  >> simp[eval_def, nice_eval_def]
+  >- (FULL_CASE_TAC >> gvs[] >> cheat)
+  >> cheat
+     (* OPT_MMAP_CONG *)
+QED
+*)
+
+(*
+
+
+Theorem IN_SINGLETON_SUBSET:
+  ∀a X. a ∈ X ⇒ {a} ⊆ X
+Proof rw[]
+QED
+
 (* The types representing local variables and memory in the semantics. *)
 (* XXX: I don't like type names conflicting with variable names. I think we can
         just delete these. *)
@@ -143,7 +595,7 @@ Definition range_def:
                 e)
     | locals, memory | (locals, memory) ∈ ctxt.locals_memory }
 End
-
+∈
 (* Find an upper bound on the working set of an expression. *)
 Definition working_set_exp_def:
   working_set_exp (Const w) ctxt = ({}:'a word set) ∧
@@ -180,134 +632,4 @@ Definition context_union_def:
 End
 
 (* Find an upper bound on the working set of a program. *)
-Definition working_set_def:
-  working_set (Skip:'a panLang$prog) (ctxt:('a, 'ffi) context) = (ctxt, {}) ∧
-  working_set (Dec v e p) ctxt =
-    (let ws = working_set_exp e ctxt and
-         values = range e ctxt;
-         lm = { (locals |+ (v, value), memory)
-              | (locals, memory) ∈ ctxt.locals_memory ∧ value ∈ values };
-         ctxt' = ctxt with locals_memory := lm;
-         (ctxt'', ws') = working_set p ctxt' in
-      (ctxt'', ws ∪ ws')) ∧
-  working_set (Assign v e) ctxt =
-    (let ws = working_set_exp e ctxt and
-         values = range e ctxt;
-         lm = { (locals |+ (v, value), memory)
-              | (locals, memory) ∈ ctxt.locals_memory ∧ value ∈ values } in
-      (ctxt with locals_memory := lm, ws)) ∧
-  working_set (Store dst src) ctxt =
-    (let ws = working_set_exp dst ctxt and
-         ws' = working_set_exp src ctxt and
-         addrs = { addr | ValWord addr ∈ range dst ctxt } and
-         values = range src ctxt;
-         lm = { (locals, THE (mem_stores addr (flatten value) UNIV memory))
-              | (locals, memory) ∈ ctxt.locals_memory ∧ addr ∈ addrs ∧
-                value ∈ values} in
-      (ctxt with locals_memory := lm, ws ∪ ws' ∪ addrs)) ∧
-  working_set (StoreByte dst src) ctxt =
-    (let ws = working_set_exp dst ctxt and
-         ws' = working_set_exp src ctxt and
-         addrs = { addr | ValWord addr ∈ range dst ctxt } and
-         ws = { w | ValWord w ∈ range src ctxt };
-         lm = { (locals, THE (mem_store_byte memory UNIV ctxt.be addr (w2w w)))
-              | locals, memory, addr, w
-              | (locals, memory) ∈ ctxt.locals_memory ∧ addr ∈ addrs ∧
-                w ∈ ws} in
-      (ctxt with locals_memory := lm, ws ∪ ws' ∪ addrs)) ∧
-  working_set (Seq c1 c2) ctxt =
-    (let (ctxt', ws) = working_set c1 ctxt;
-        (ctxt'', ws') = working_set c2 ctxt' in
-      (ctxt'', ws ∪ ws')) ∧
-  working_set (If e c1 c2) ctxt =
-    (let ws = working_set_exp e ctxt and
-        (ctxt', ws') = working_set c1 ctxt and
-        (ctxt'', ws'') = working_set c2 ctxt in
-      (context_union ctxt' ctxt'', ws ∪ ws' ∪ ws'')) ∧
-  (* For the purposes of defining the major theorem below, this is sound because
-     the nice semantics are the same as the semantics for While. This saves us
-     a huge headache, but restricts working_set to finding the bound up until
-     the next While loop. *)
-  working_set (While _ _) ctxt = (ctxt, {}) ∧
-  working_set Break ctxt = (ctxt, {}) ∧
-  working_set Continue ctxt = (ctxt, {}) ∧
-  (* See the note above on the While case. *)
-  working_set (Call _ _ _) ctxt = (ctxt, {}) ∧
-  (* See the note above on the While case. *)
-  working_set (ExtCall _ _ _ _ _) ctxt = (ctxt, {}) ∧
-  working_set (Return e) ctxt = (ctxt, working_set_exp e ctxt) ∧
-  working_set (Raise eid e) ctxt = (ctxt, working_set_exp e ctxt) ∧
-  working_set Tick ctxt = (ctxt, {})
-End
-
-
-(* Prove the major theorem: that if our bound on the working set of a Pancake
-   program is within the allocated heap, we may replace the semantics with the
-   nicer semantics. *)
-
-Theorem foo:
-  THE (eval s e) ∈ range e (state_to_context s)
-Proof
-  cheat
-QED
-
-Theorem working_set_mono:
-  s.locals_memory ⊆ lm ⇒ 
-  SND (working_set p s) ⊆ SND (working_set p (s with locals_memory := lm))
-Proof
-  cheat
-QED
-
-(* Useful with DEP_PURE_ONCE_REWRITE_TAC. *)
-Theorem no_out_of_bounds:
-  ∀p s.
-    SND (working_set p (state_to_context s)) ⊆ s.memaddrs ⇒
-    evaluate (p, s) = nice_evaluate (p, s)
-Proof
-  recInduct panSemTheory.evaluate_ind
-  >> rpt strip_tac
-    >- simp[evaluate_def, nice_evaluate_def]
-    >- (simp[evaluate_def, nice_evaluate_def]
-      >> TOP_CASE_TAC
-      >> AP_TERM_TAC
-      >> first_x_assum $ match_mp_tac o MP_CANON
-      >> simp[]
-      >> last_x_assum mp_tac
-      >> simp[working_set_def, state_to_context_def]
-      >> qmatch_goalsub_abbrev_tac `SND (_ a) ⊆ _ ⇒ SND b ⊆ _`
-
-      >> Q.SUBGOAL_THEN `SND b ⊆ SND a` assume_tac
-
-
-      >> subgoal `SND b ⊆ SND a`
-      >> `SND b ⊆ SND a` suffices_by (simp[SUBSET_DEF,ELIM_UNCURRY,IN_DEF])
-
-
-      >> last_x_assum mp_tac
-      >> simp[state_to_context_def, working_set_def]
-      >> qmatch_goalsub_abbrev_tac ‘SND(_ a1) ⊆ _ ⇒ SND a2 ⊆ _’
-      >> ‘SND a2 ⊆ SND a1’ suffices_by (simp[SUBSET_DEF,ELIM_UNCURRY,IN_DEF])
-      >> MAP_EVERY qunabbrev_tac [‘a1’,‘a2’]
-
-
-      >> simp[state_to_context_def]
-      >> simp[working_set_def]
-      >> ``
-
-
-      >> EVAL_TAC
-      >> simp[]
-
-      >> cheat)
-  >> rpt cheat
-QED
-
-(* ways of simplifying an assumption:
-     >> last_x_assum $ assume_tac o SRULE[working_set_def]
-fs[working_set_def]
-
-thanks gordon *)
-
-
-val _ = export_theory ();
-
+d*)
